Clean up and documentation of equ

theories/Equ.v
@@ -1,35 +1,45 @@
-(* begin hide *)
+(*|
+==============================
+Syntactic equality over ctrees
+==============================
+As always with coinductive structures in Coq, [eq] is too strong
+to be usable. We hence define through this file [equ], a coinductive
+syntactic equality over the structure. [equ] enforces the trees to
+have the exact same shape, constructor by constructor.
+
+This relation is analogous to what is dubbed as _strong bisimulation_
+for [itree], but we are trying to avoid this terminology here since
+we reserve the notion of bisimulation for the equivalence relations
+that take internal non-determinism into account.
+
+|*)
 From Coq Require Import RelationClasses Program.
 
 From Coinduction Require Import
 	coinduction rel tactics.
 
 From CTree Require Import
-	 Utils
+	   Utils
      CTrees
      Shallow.
-(* end hide *)
-
-(** * Structural equality of [ctree]s
-	Analogous to what is dubbed as _strong bisimulation_
-	for [ctree], but trying to avoid this terminology here
-	to reserve the notion of bisimulation for the equivalence
-	relation that takes internal non-determinism into account.
-*)
+(*|
+.. coq:
+|*)
 
 Section equ.
 
   Context {E : Type -> Type} {R1 R2 : Type} (RR : R1 -> R2 -> Prop).
 
-  (** We also need to do some gymnastics to work around the
-      two-layered definition of [ctree]. We first define a
-      relation transformer [eqitF] as an indexed inductive type
-      on [ctreeF], which is then composed with [observe] to obtain
-      a relation transformer on [ctree] ([eqit_]).
+(*|
+We also need to do some gymnastics to work around the
+two-layered definition of [ctree]. We first define a
+relation transformer [equF] as an indexed inductive type
+on [ctree'], which is then composed with [observe] to obtain
+a relation transformer on [ctree] ([equ_]).
 
-      In short, this is necessitated by the fact that dependent
-      pattern-matching is not allowed on [ctree].
-   *)
+In short, this is necessitated by the fact that dependent
+pattern-matching is not allowed on [ctree].
+|*)
 
   Variant equF (eq : ctree E R1 -> ctree E R2 -> Prop) :
     ctree' E R1 -> ctree' E R2 -> Prop :=
@@ -54,16 +64,36 @@ Section equ.
 
 End equ.
 
-(** associated relation *)
+(*|
+The relation itself, defined as the greatest fixed-point of [fequ].
+Through this development, we use the [coinduction] package developed
+by Damien Pous to define and reason about coinductive relations.
+The approach is based on the so-called "companion", described in
+the paper "Coinduction All the Way Up" (Pous, LICS'16).
+
+The greastest fixed-point is defined by the construction [gfp].
+It gives access to the following tactics:
+- [coinduction S CIH] initiates a coinductive proof;
+- [step in H] unfold in [H] the [gfp], exposing here for instance
+[equF], allowing for an inversion to be performed;
+- [step] unfolds in the goal the [gfp], exposing [equF], so that
+one can play the game once. Note that formally speaking, this
+corresponds to reasoning "up-to fequ".
+- additionnaly, the companion provides extensive support for
+up-to reasoning: any function [f] proved to be below the companion,
+denoted [t], is accessible during a proof by coinduction.
+
+|*)
 Notation equ R := (gfp (fequ R)).
 Infix "≅" := (equ eq) (at level 70).
 
-(** associated companions  *)
-Notation T_equ RR  := (t (B (fequ RR))).
+(*|
+The associated companions:
+|*)
+Notation T_equ RR  := (T (fequ RR)).
 Notation t_equ RR  := (t (fequ RR)).
 Notation bt_equ RR := (bt (fequ RR)).
 Arguments equ_ _ _ _ _/.
-Ltac desobs x := destruct (observe x) .
 #[global] Hint Constructors equF: core.
 
 Section equ_equiv.
@@ -72,35 +102,42 @@ Section equ_equiv.
   Notation T  := (coinduction.T (fequ (E := E) RR)).
   Notation t  := (coinduction.t (fequ (E := E) RR)).
   Notation bt := (coinduction.bt (fequ (E := E) RR)).
+(*|
+This is just a hack suggested by Damien Pous to avoid a
+universe inconsistency when using both the relational algebra
+and coinduction libraries (we fix the type at which we'll use [eq]).
+|*)
   Definition seq: relation (ctree E R) := eq.
 
-  (** [eq] is a post-fixpoint, thus [const eq] is below [t] *)
-	Lemma refl_t {RRR: Reflexive RR}: const seq <= t.
+(*|
+[eq] is a post-fixpoint, thus [const eq] is below [t]
+These kind of lemmas are proofs of validity of up-to reasoning
+principles: [t_equ RR] is the companion of the monotone function
+[fequ RR]. By proving that the function (on relations over ctrees)
+[const seq] (i.e. [fun R => eq]) is below the companion, it is proved
+to be a valid enhancement, and hence can be used at any point during
+a coinductive proof.
+Here concretely, bisimulation candidates don't ever need
+to be closed by reflexivity in effect: the companion is always reflexive.
+|*)
+	Lemma refl_t {RRR: Reflexive RR}: const seq <= t_equ RR.
 	Proof.
 		apply leq_t. intro.
 		change (@eq (ctree E R)  <= equ_ RR eq).
 		intros p ? <-. cbn. desobs p; auto.
 	Qed.
 
-	(** converse is compatible *)
+(*|
+[converse] is compatible: up-to symmetry is valid
+|*)
 	Lemma converse_t {RRS: Symmetric RR}: converse <= t.
 	Proof.
 		apply leq_t. intros S x y H; cbn. destruct H; auto.
 	Qed.
 
-	Lemma Vis_eq1 T Y e k Z f h: @VisF E R T Y e k = @VisF E R T Z f h -> Y=Z.
-	Proof. intro H. now dependent destruction H. Qed.
-
-	Lemma Vis_eq2 T Y e k f h: @VisF E R T Y e k = @VisF E R T Y f h -> e=f /\ k=h.
-	Proof. intro H. now dependent destruction H. Qed.
-
-	Lemma Choice_eq1 T b b' n m k h: @ChoiceF E R T b n k = @ChoiceF E R T b' m h -> b = b' /\ n=m.
-	Proof. intro H. now dependent destruction H. Qed.
-
-	Lemma Choice_eq2 T b n k h: @ChoiceF E R T b n k = @ChoiceF E R T b n h -> k=h.
-	Proof. intro H. now dependent destruction H. Qed.
-
-	(** so is squaring *)
+(*|
+[squaring] is compatible: up-to transitivity is valid
+|*)
 	Lemma square_t {RRR: Reflexive RR} {RRT: Transitive RR}: square <= t.
 	Proof.
 		apply leq_t.
@@ -108,25 +145,34 @@ Section equ_equiv.
 		inversion xy; inversion yz; try (exfalso; congruence).
 		- constructor. replace y0 with x1 in * by congruence. eauto.
 		- rewrite <-H in H2.
-			destruct (Vis_eq1 _ _ _ _ _ _ _ H2).
-			destruct (Vis_eq2 _ _ _ _ _ _ H2) as [-> ->].
+			destruct (Vis_eq1 H2).
+			destruct (Vis_eq2 H2) as [-> ->].
 			constructor. intro x0. now exists (k2 x0).
 		- rewrite <- H in H2.
-			destruct (Choice_eq1 _ _ _ _ _ _ _ H2); subst.
-			destruct (Choice_eq2 _ _ _ _ _ H2).
+			destruct (Choice_eq1 H2); subst.
+			destruct (Choice_eq2 H2).
 			constructor. intros i. now (exists (k0 i)).
 	Qed.
 
-	(** thus bisimilarity, [t R], [b (t R)] and [T f R] are always equivalence relations *)
+(*|
+Having [const eq], [converse] and [square] below the companion entails respectively
+that the companion, at all point, is reflexive, symmetric, transitive.
+The companion library directly provide these results for bisimilarity, [t R], [b (t R)]
+and [T f R].
+|*)
 	#[global] Instance Equivalence_et `{Equivalence _ RR} S: Equivalence (t S).
 	Proof. apply Equivalence_t. apply refl_t. apply square_t. apply converse_t. Qed.
 	#[global] Instance Equivalence_T `{Equivalence _ RR} f S: Equivalence (T f S).
-	Proof.
-    apply Equivalence_T. apply refl_t. apply square_t. apply converse_t. Qed.
+	Proof. apply Equivalence_T. apply refl_t. apply square_t. apply converse_t. Qed.
 	#[global] Instance Equivalence_bt `{Equivalence _ RR} S: Equivalence (bt S).
 	Proof. apply Equivalence_bt. apply refl_t. apply square_t. apply converse_t. Qed.
 
-	(* This one is a bit annoyingly adhoc, but useful for unfolding laws *)
+(*|
+This instance is a bit annoyingly adhoc, but useful for unfolding laws notably:
+essentially we can conclude by reflexivity without stepping completely through
+[equF], but only after exposing it by unfolding and case-analysing on the structure
+of the tree.
+|*)
   #[global] Instance Reflexive_equF (equ : ctree E R -> ctree E R -> Prop) :
     Reflexive RR -> Reflexive equ -> Reflexive (equF RR equ).
   Proof.
@@ -141,15 +187,17 @@ Proof. apply Equivalence_et. typeclasses eauto. Qed.
 #[global] Hint Constructors equF : core.
 Arguments equ_ {E R1 R2} RR eq t1 t2/.
 
-(* We assume JMeq to invert easily bisimilarity of dependently
-	 typed constructors *)
+(*|
+Dependent inversion of [equ] and [equF] equations
+-------------------------------------------------
+We assume [JMeq_eq] to invert easily bisimilarity of dependently typed constructors
+|*)
 Lemma equ_vis_invT {E X Y S} (e1 : E X) (e2 : E Y) (k1 : X -> ctree E S) k2 :
   Vis e1 k1 ≅ Vis e2 k2 ->
   X = Y.
 Proof.
   intros EQ.
-
-	step in EQ. cbn in *; dependent induction EQ; auto.
+	step in EQ. dependent induction EQ; auto.
 Qed.
 
 Lemma equ_vis_invE {E X S} (e1 e2 : E X) (k1 k2 : X -> ctree E S) :
@@ -158,15 +206,13 @@ Lemma equ_vis_invE {E X S} (e1 e2 : E X) (k1 k2 : X -> ctree E S) :
 Proof.
   intros EQ; step in EQ.
 	inv EQ.
-	dependent destruction H1.
 	dependent destruction H2.
-	dependent destruction H.
 	dependent destruction H4.
 	auto.
 Qed.
 
 Lemma equF_vis_invT {E X Y S} (e1 : E X) (e2 : E Y) (k1 : X -> ctree E S) k2 :
-  equF eq (equ eq) (CTrees.VisF e1 k1) (CTrees.VisF e2 k2) ->
+  equF eq (equ eq) (VisF e1 k1) (VisF e2 k2) ->
   X = Y.
 Proof.
   intros EQ.
@@ -174,7 +220,7 @@ Proof.
 Qed.
 
 Lemma equF_vis_invE {E X S} (e1 e2 : E X) (k1 k2 : X -> ctree E S) :
-  equF eq (equ eq) (CTrees.VisF e1 k1) (CTrees.VisF e2 k2) ->
+  equF eq (equ eq) (VisF e1 k1) (VisF e2 k2) ->
   e1 = e2 /\ forall x, equ eq (k1 x) (k2 x).
 Proof.
   intros EQ.
@@ -183,7 +229,7 @@ Proof.
 Qed.
 
 Lemma equF_choice_invT {E S b b' n m} (k1 : _ -> ctree E S) k2 :
-  equF eq (equ eq) (CTrees.ChoiceF b n k1) (CTrees.ChoiceF b' m k2) ->
+  equF eq (equ eq) (ChoiceF b n k1) (ChoiceF b' m k2) ->
   n = m /\ b = b'.
 Proof.
   intros EQ.
@@ -191,13 +237,27 @@ Proof.
 Qed.
 
 Lemma equF_choice_invE {E S b n} (k1 : _ -> ctree E S) k2 :
-  equF eq (equ eq) (CTrees.ChoiceF b n k1) (CTrees.ChoiceF b n k2) ->
+  equF eq (equ eq) (ChoiceF b n k1) (ChoiceF b n k2) ->
   forall x, equ eq (k1 x) (k2 x).
 Proof.
   intros EQ.
 	inv EQ.
 	dependent destruction H; auto.
 Qed.
+
+(*|
+Proper Instances
+----------------
+TODO: step back and think a bit better about those
+
+equ eq       ==> going (equ eq)  observe
+∀(equ eq)    ==> going (equ eq)  ChoiceF
+∀(equ eq)    ==> going (equ eq)  VisF
+observing eq --> equ eq
+going(equ)   ==> eq ==> fimpl    equF eq (t_equ eq r)
+eq ==> going(equ)   ==> fimpl    equF eq (t_equ eq r)
+equ ==> equ ==> flip impl)       bt_equ eq r
+|*)
 
 #[global] Instance equ_observe {E R} :
   Proper (equ eq ==> going (equ eq)) (@observe E R).
@@ -225,8 +285,8 @@ Proof.
 Qed.
 
 #[global] Instance equ_eq_equF {E R r} :
-  Proper (going (gfp (@fequ E R R eq)) ==> eq ==> flip impl)
-	     (equF eq (t_equ eq r)).
+  Proper (going (equ eq) ==> eq ==> flip impl)
+	     (@equF E R R eq (t_equ eq r)).
 Proof.
   unfold Proper, respectful, flip, impl. intros. subst.
   inv H. step in H0. inv H0; inv H1; auto.
@@ -237,8 +297,8 @@ Proof.
 Qed.
 
 #[global] Instance eq_equ_equF {E R r} :
-  Proper (eq ==> going (gfp (@fequ E R R eq)) ==> flip impl)
-	     (equF eq (t_equ eq r)).
+  Proper (eq ==> going (equ eq) ==> flip impl)
+	     (@equF E R R eq (t_equ eq r)).
 Proof.
   unfold Proper, respectful, flip, impl. intros. subst.
   inv H0. step in H. inv H; inv H1; auto.
@@ -249,7 +309,7 @@ Proof.
 Qed.
 
 #[global] Instance gfp_bt_equ {E R r} :
-	 Proper (gfp (@fequ E R R eq) ==> gfp (@fequ E R R eq) ==> flip impl)
+	 Proper (gfp (@fequ E R R eq) ==> equ eq ==> flip impl)
 	  (bt_equ eq r).
 Proof.
 	unfold Proper, respectful, flip, impl.
@@ -260,11 +320,23 @@ Proof.
 	apply H2; symmetry; assumption.
 Qed.
 
-(* Elementary equational theory *)
+(*|
+Elementary equational theory
+----------------------------
+At this point, equipped with our coinductive structural equality,
+we can already express tight equations. Mainly
+- unfolding lemmas for our operations ([bind] and [iter] notably);
+- up-to bind coinductive principle for [equ];
+- the three monadic laws
+|*)
 Import CTree.
 Import CTreeNotations.
 Open Scope ctree.
 
+(*|
+Even eta-laws for coinductive data-structures are not valid w.r.t. to [eq]
+in Coq. We however do recover them w.r.t. [equ].
+|*)
 Lemma ctree_eta_ {E R} (t : ctree E R) : t ≅ go (_observe t).
 Proof. now step. Qed.
 
@@ -291,24 +363,50 @@ Proof.
 	now step.
 Qed.
 
+Notation iter_ step i :=
+  (lr <- step i;;
+   match lr with
+   | inl l => TauI (iter step l)
+   | inr r => Ret r
+   end)%ctree.
+
 Lemma unfold_iter {E R I} (step : I -> ctree E (I + R)) i:
-	iter step i ≅
-       lr <- step i;;
-  match lr with
-  | inl l => TauI (iter step l)
-  | inr r => Ret r
-  end.
+	iter step i ≅ iter_ step i.
 Proof.
 	now step.
 Qed.
 
+(*|
+Up-to bind principle
+~~~~~~~~~~~~~~~~~~~~
+Consider two computations explicitely built as sequences
+[t >>= k] and [u >>= l]. When trying to prove that they are
+bisimilar via a coinductive proof, one is faced with a goal
+of the shape:
+[t_equ RR r (t >>= k) (u >>= l)]
+One can of course case analysis on the structure of [t] and [u]
+to make progress in the proof.
+But if we know from another source that [t ≅ u], we would like
+to be able to simply "match" these prefixes, and continue the
+coinductive proof over the continuations.
+Such a reasoning is dubbed "up-to bind" reasoning, which we
+prove sound in the following.
 
+More formally, this corresponds as always to establishing that
+the appropriate function is a valid enhancement. The function
+in question here is:
+f R = {(bind t k, bind u l) | equ SS t u /\ forall x y, SS x y -> R (k x) (l x)}
+
+|*)
 Section bind.
 
+(*|
+Heterogeneous [pair], todo move to coinduction library
+|*)
   Definition pointwise {X X' Y Y'} (SS : rel X X')
     : rel Y Y' -> rel (X -> Y) (X' -> Y') :=
     fun R k k' => forall x x', SS x x' -> R (k x) (k' x').
-  (* Heterogeneous [pair], todo move to library *)
+
   Definition pairH {A B : Type} (x : A) (y : B) : A -> B -> Prop :=
     fun x' y' => x = x' /\ y = y'.
 
@@ -322,27 +420,38 @@ Section bind.
 
     Context {E: Type -> Type} {X X' Y Y': Type}.
 
-    (* Most general contextualisation function associated to [bind]
-	   Can be read more digestly as, where R is a relation on ctrees (the prefixes of the binds) and S on the continuations:
-		 bind_ctx R S = {(bind t k, bind t' k') | R t t' /\ S k k'}
+(*|
+Most general contextualisation function associated to [bind].
+Can be read more digestly as, where R is a relation on ctrees
+(the prefixes of the binds) and S on the continuations:
+bind_ctx R S = {(bind t k, bind t' k') | R t t' /\ S k k'}
 
-		 This definition could actually be generalized,
-     the same way the Coinduction library provides generic binary contexts ([binary_ctx]).
-	   *)
+Note that at this point, this is more general that what we are
+interested in: we will specialize [R] and [S] for our purpose,
+first here w.r.t. to [equ], later w.r.t. to other relations over
+[ctree]s.
 
-    (* The most general context:
-    bind_ctx R S ≜ {(bind x k, bind x' k') | R x x' /\ S k k'}
-     *)
+Remark: the Coinduction library provides generic binary contexts
+[binary_ctx], but whose both arguments are at the same types.
+We could provide an heterogeneous version of [binary_ctx] and have
+[bind_ctx] be an instance of it to avoid having to rethink in terms
+of [sup_all] locally.
+|*)
+
     Definition bind_ctx
                (R: rel (ctree E X) (ctree E X'))
                (S: rel (X -> ctree E Y) (X' -> ctree E Y')):
       rel (ctree E Y) (ctree E Y') :=
-      sup_all (fun x => sup (R x) (fun x' =>
-                                  sup_all (fun k => sup (S k) (fun k' => pairH (bind x k) (bind x' k'))))).
+      sup_all (fun x => sup (R x)
+                         (fun x' => sup_all
+                                   (fun k => sup (S k)
+                                              (fun k' => pairH (bind x k) (bind x' k'))))).
 
-    (* Two lemmas to interact with [bind_ctx]:
-     - [leq_bind_ctx] specifies relations above the context
-     - [in_bind_ctx] specifies how to populate it *)
+(*|
+Two lemmas to interact with [bind_ctx] before making it opaque:
+- [leq_bind_ctx] specifies relations above the context
+- [in_bind_ctx] specifies how to populate it
+|*)
     Lemma leq_bind_ctx:
       forall R S S', bind_ctx R S <= S' <->
                   (forall x x', R x x' -> forall k k', S k k' -> S' (bind x k) (bind x' k')).
@@ -360,15 +469,24 @@ Section bind.
     Lemma in_bind_ctx (R S :rel _ _) x x' y y':
       R x x' -> S y y' -> bind_ctx R S (bind x y) (bind x' y').
     Proof. intros. now apply ->leq_bind_ctx. Qed.
-    Global Opaque bind_ctx.
+    #[global] Opaque bind_ctx.
 
   End Bind_ctx.
 
+(*|
+Specialization of [bind_ctx] to the [equ]-based closure we are
+looking for, and the proof of validity of the principle. As
+always with the companion, we prove that it is valid by proving
+that it si below the companion.
+|*)
   Section Concrete_Bind_ctx.
 
     Context {E: Type -> Type} {X1 X2 Y1 Y2: Type}.
 
-    (* specialisation to a function acting with [equ] on the bound value, and with the argument (pointwise) on the continuation *)
+(*|
+Specialization of [bind_ctx] to a function acting with [equ] on the bound value,
+and with the argument (pointwise) on the continuation.
+|*)
     Program Definition bind_ctx_equ SS: mon (rel (ctree E Y1) (ctree E Y2)) :=
       {|body := fun R => @bind_ctx E X1 X2 Y1 Y2 (equ SS) (pointwise SS R) |}.
     Next Obligation.
@@ -376,7 +494,9 @@ Section bind.
       apply in_bind_ctx. apply H'. intros t t' HS. apply H0, H'', HS.
     Qed.
 
-    (* this gives a valid up-to technique *)
+(*|
+The resulting enhancing function gives a valid up-to technique
+|*)
     Lemma bind_ctx_equ_t (SS : rel X1 X2) (RR : rel Y1 Y2): bind_ctx_equ SS <= t_equ RR.
     Proof.
       apply Coinduction. intros R. apply (leq_bind_ctx _).
@@ -400,6 +520,9 @@ Section bind.
 
 End bind.
 
+(*|
+Expliciting the reasoning rule provided by the up-to principle.
+|*)
 Lemma equ_clo_bind (E: Type -> Type) (X1 X2 Y1 Y2 : Type) :
 	forall (t1 : ctree E X1) (t2 : ctree E X2) (k1 : X1 -> ctree E Y1) (k2 : X2 -> ctree E Y2)
     (S : rel X1 X2) (R : rel Y1 Y2) RR,
@@ -413,7 +536,10 @@ Proof.
   now apply in_bind_ctx.
 Qed.
 
-(* and as a consequence, one may rewrite under binds *)
+(*|
+And in particular, we get the proper instance justifying rewriting [equ]
+to the left of a [bind].
+|*)
 #[global] Instance bind_equ_cong :
  forall (E : Type -> Type) (X Y : Type) (R : rel Y Y) RR,
    Proper (equ (@eq X) ==> pointwise_relation X (t_equ R RR) ==> t_equ R RR) (@bind E X Y).
@@ -422,6 +548,11 @@ Proof.
   intros ? ? <-; auto.
 Qed.
 
+(*|
+Monadic laws
+------------
+The three usual monadic laws can be estalished w.r.t. [equ eq].
+|*)
 Lemma bind_ret_l {E X Y} : forall (x : X) (k : X -> ctree E Y),
     Ret x >>= k ≅ k x.
 Proof.
